
    \documentclass{article}
    \usepackage{amsfonts}
    \usepackage{amsmath,multicol,eso-pic}
    \begin{document}
    \title{Algebra 101 worksheet 1 Solutions} 
 \date{\vspace{-5ex}} 
 \maketitle

        \section{Linear equations}
        
        \begin{enumerate}
        \item$$a =\frac{g - 5}{H - 14}$$
\item$$N =\frac{16}{- S + w}$$
\item$$A =\frac{h + 4}{E - 6}$$
\item$$w =\frac{z}{15} - \frac{23}{15}$$
\item$$b =\frac{K - 5}{Y - 23}$$
\item$$M =\frac{10}{S - 4}$$
\item$$y =\frac{- V + z}{T - X}$$
\item$$p =\frac{6}{Q + 2}$$
\item$$p =\frac{- V + g}{t + 5}$$
\item$$H =\frac{y - 20}{E - u}$$
\item$$M =\frac{R + 10}{R - k}$$
\item$$M =\frac{- b + 9}{j + 26}$$
\item$$V =\frac{P - X}{Q - S}$$
\item$$P =- \frac{e}{13} + \frac{1}{13}$$
\item$$g =- \frac{37}{7}$$
\item$$K =\frac{S + 6}{T + 23}$$
\item$$d =\frac{Q + 24}{N + 10}$$
\item$$D =- \frac{27}{m - 8}$$
\item$$E =\frac{- y + 2}{q + 5}$$
\item$$r =\frac{c - 10}{x + 5}$$
        \end{enumerate}
        

        \section{Quadratic equations}
        
        \begin{enumerate}
        \item$$y = - \frac{15}{8} - \frac{\sqrt{65}}{8}, y = - \frac{15}{8} + \frac{\sqrt{65}}{8}$$
\item$$x = \frac{19}{18} + \frac{\sqrt{757}}{18}, x = - \frac{\sqrt{757}}{18} + \frac{19}{18}$$
\item$$x = -10, x = 23$$
\item$$y = \frac{1}{4} + \frac{\sqrt{177}}{4}, y = - \frac{\sqrt{177}}{4} + \frac{1}{4}$$
\item$$x = 0, x = 22$$
\item$$x = \frac{8}{13} - \frac{3 i}{13} \sqrt{29}, x = \frac{8}{13} + \frac{3 i}{13} \sqrt{29}$$
\item$$x = -2, x = 10$$
\item$$x = - \frac{1}{22} + \frac{\sqrt{309}}{22}, x = - \frac{\sqrt{309}}{22} - \frac{1}{22}$$
\item$$x = 0, x = \frac{24}{5}$$
\item$$y = - \frac{11}{20} - \frac{\sqrt{799} i}{20}, y = - \frac{11}{20} + \frac{\sqrt{799} i}{20}$$
\item$$x = 0, x = \frac{4}{15}$$
\item$$x = 12, x = 15$$
\item$$y = 2, y = 6$$
\item$$x = -17, x = 23$$
\item$$x = -7, x = -1$$
\item$$x = -13, x = -5$$
\item$$x = -3, x = \frac{7}{4}$$
\item$$x = \frac{5}{21} + \frac{2 \sqrt{85}}{21}, x = - \frac{2 \sqrt{85}}{21} + \frac{5}{21}$$
\item$$y = \frac{25}{26} + \frac{\sqrt{1041}}{26}, y = - \frac{\sqrt{1041}}{26} + \frac{25}{26}$$
\item$$x = 0, x = 1$$
        \end{enumerate}
        

        \section{Compute the derivative}
        
        \begin{enumerate}
        \item$$\frac{1}{x} \left(14 x + 12\right) - \frac{1}{x^{2}} \left(7 x^{2} + 12 x - 24\right)$$
\item$$\frac{2 \sqrt{x} \left(27 x^{2} - 18\right)}{\left(- 9 x^{3} + 18 x + 7\right)^{2}} + \frac{1}{\sqrt{x} \left(- 9 x^{3} + 18 x + 7\right)}$$
\item$$\frac{1}{\left(16 x^{3} - 23 x^{2} + 5 x\right)^{2}} \left(\log{\left (x \right )} + \tan{\left (x \right )}\right) \left(- 48 x^{2} + 46 x - 5\right) + \frac{\tan^{2}{\left (x \right )} + 1 + \frac{1}{x}}{16 x^{3} - 23 x^{2} + 5 x}$$
\item$$- \left(e^{x} + \tan{\left (x \right )}\right) e^{- x} + \left(e^{x} + \tan^{2}{\left (x \right )} + 1\right) e^{- x}$$
\item$$- \left(19 x + e^{x}\right) e^{- x} + \left(e^{x} + 19\right) e^{- x}$$
\item$$\frac{1}{x} \left(48 x - \sin{\left (x \right )} + 7\right) - \frac{1}{x^{2}} \left(24 x^{2} + 7 x + \cos{\left (x \right )}\right)$$
\item$$\frac{1}{\tan^{2}{\left (x \right )}} \left(\log{\left (x \right )} + \sin{\left (x \right )}\right) \left(- \tan^{2}{\left (x \right )} - 1\right) + \frac{\cos{\left (x \right )} + \frac{1}{x}}{\tan{\left (x \right )}}$$
\item$$\frac{1}{x} \left(12 x^{2} + \frac{1}{x}\right) - \frac{1}{x^{2}} \left(4 x^{3} + \log{\left (x \right )} - 17\right)$$
\item$$\frac{1}{\sin{\left (x \right )}} \left(- 51 x^{2} + 48 x + 14 + \frac{1}{x}\right) - \frac{\cos{\left (x \right )}}{\sin^{2}{\left (x \right )}} \left(- 17 x^{3} + 24 x^{2} + 14 x + \log{\left (x \right )} - 14\right)$$
\item$$\left(\frac{1}{x} + \frac{1}{2 \sqrt{x}}\right) e^{- x} - \left(\sqrt{x} + \log{\left (x \right )}\right) e^{- x}$$
        \end{enumerate}
        

    \end{document}
    