
    \documentclass{article}
    \usepackage{amsfonts}
    \usepackage{amsmath,multicol,eso-pic}
    \begin{document}
    \title{Example Worksheet 1 Solutions} 
 \date{\vspace{-5ex}} 
 \maketitle

        \section{Linear equations}
        
        \begin{enumerate}
        \item$$E =\frac{- T + 23}{F + 15}$$
\item$$q =\frac{E - 15}{T + 12}$$
\item$$v =\frac{y + 15}{f - 18}$$
\item$$x =- \frac{21}{H + 5}$$
\item$$n =\frac{c - 12}{B + 11}$$
\item$$b =\frac{- A + g}{T - 11}$$
\item$$X =- \frac{a}{13} - 1$$
\item$$b =\frac{h + 2}{- T + z}$$
\item$$d =- \frac{j + 3}{K - 10}$$
\item$$q =\frac{g}{13} - \frac{r}{13}$$
\item$$d =\frac{- A + 21}{S - r}$$
\item$$u =- \frac{15}{28}$$
\item$$Y =- \frac{E}{6} - \frac{17}{6}$$
\item$$j =- \frac{14}{t + 13}$$
\item$$W =\frac{- C + c}{g + 26}$$
\item$$r =\frac{t + 2}{H + 19}$$
\item$$N =- \frac{18}{31}$$
\item$$v =- \frac{11}{37}$$
\item$$d =- \frac{9}{8}$$
\item$$x =- \frac{S + 25}{N - W}$$
        \end{enumerate}
        

        \section{Quadratic equations}
        
        \begin{enumerate}
        \item$$y = - \frac{1}{16} + \frac{\sqrt{769}}{16}, y = - \frac{\sqrt{769}}{16} - \frac{1}{16}$$
\item$$y = - \frac{1}{2} - \frac{3 i}{10} \sqrt{10}, y = - \frac{1}{2} + \frac{3 i}{10} \sqrt{10}$$
\item$$x = - \frac{1}{26} - \frac{\sqrt{467} i}{26}, x = - \frac{1}{26} + \frac{\sqrt{467} i}{26}$$
\item$$y = -22, y = -6$$
\item$$x = 16, x = 23$$
\item$$x = 3, x = 14$$
\item$$x = -26, x = 20$$
\item$$y = -26, y = 14$$
\item$$y = 11, y = 21$$
\item$$y = 0, y = \frac{24}{17}$$
\item$$y = -6, y = -2$$
\item$$y = -14, y = 22$$
\item$$x = - \frac{2}{3} + \frac{\sqrt{226}}{6}, x = - \frac{\sqrt{226}}{6} - \frac{2}{3}$$
\item$$y = \frac{2}{43} + \frac{\sqrt{262}}{43}, y = - \frac{\sqrt{262}}{43} + \frac{2}{43}$$
\item$$x = 7, x = 11$$
\item$$x = -19, x = 13$$
\item$$y = 4, y = 23$$
\item$$y = - \frac{1}{14} - \frac{3 i}{14} \sqrt{31}, y = - \frac{1}{14} + \frac{3 i}{14} \sqrt{31}$$
\item$$x = - \frac{5}{4}, x = 0$$
\item$$x = -26, x = 8$$
        \end{enumerate}
        

        \section{Differentiation}
        
        \begin{enumerate}
        \item$$\frac{e^{x} + \frac{1}{x}}{\tan{\left (x \right )}} + \frac{1}{\tan^{2}{\left (x \right )}} \left(e^{x} + \log{\left (x \right )}\right) \left(- \tan^{2}{\left (x \right )} - 1\right)$$
\item$$- \left(\sqrt{z} + \sin{\left (z \right )}\right) e^{- z} + \left(\cos{\left (z \right )} + \frac{1}{2 \sqrt{z}}\right) e^{- z}$$
\item$$\frac{- 10 y + 1}{\tan{\left (y \right )}} + \frac{1}{\tan^{2}{\left (y \right )}} \left(- \tan^{2}{\left (y \right )} - 1\right) \left(- 5 y^{2} + y - 21\right)$$
\item$$\left(- 48 y^{2} + \cos{\left (y \right )} - 19\right) e^{- y} - \left(- 16 y^{3} - 19 y + \sin{\left (y \right )} + 23\right) e^{- y}$$
\item$$\frac{\left(46 z - 11\right) \left(\sqrt{z} - 10 z^{3} + 15 z^{2} + z\right)}{\left(- 23 z^{2} + 11 z + 12\right)^{2}} + \frac{- 30 z^{2} + 30 z + 1 + \frac{1}{2 \sqrt{z}}}{- 23 z^{2} + 11 z + 12}$$
\item$$- \frac{1}{11 x^{2}} \left(- \sin{\left (x \right )} + \frac{1}{x}\right) + \frac{2}{11 x^{3}} \left(\log{\left (x \right )} + \cos{\left (x \right )}\right)$$
\item$$\frac{\left(y + e^{y}\right) \left(- 51 y^{2} + 24\right)}{\left(17 y^{3} - 24 y - 10\right)^{2}} + \frac{e^{y} + 1}{17 y^{3} - 24 y - 10}$$
\item$$- \left(z + \tan{\left (z \right )}\right) e^{- z} + \left(\tan^{2}{\left (z \right )} + 2\right) e^{- z}$$
\item$$\frac{1}{- 8 y + 5} \left(\cos{\left (y \right )} + \tan^{2}{\left (y \right )} + 1\right) + \frac{8 \left(\sin{\left (y \right )} + \tan{\left (y \right )}\right)}{\left(- 8 y + 5\right)^{2}}$$
\item$$\frac{18 y^{2} + 72 y}{\sin{\left (y \right )}} - \frac{\cos{\left (y \right )}}{\sin^{2}{\left (y \right )}} \left(6 y^{3} + 36 y^{2}\right)$$
        \end{enumerate}
        

        \section{Compute the integral}
        
        \begin{enumerate}
        \item$$- 7 z + C $$
\item$$9 y^{2} + C $$
\item$$- \frac{13 z^{2}}{2} - 22 z + C $$
\item$$2 z + C $$
\item$$- \frac{17 y^{4}}{4} - \frac{20 y^{3}}{3} - 26 y + C $$
\item$$\frac{25 y^{2}}{2} - y + C $$
\item$$- \frac{23 y^{2}}{2} + C $$
\item$$4 z^{4} - 6 z^{2} + C $$
\item$$4 z^{2} + 6 z + C $$
\item$$5 z + C $$
        \end{enumerate}
        

        \section{Compute the integral}
        
        \begin{enumerate}
        \item$$\frac{64 y^{\frac{8}{3}}}{3} - \frac{161 y^{\frac{7}{3}}}{45} + C $$
\item$$\frac{7}{18 \sqrt{z}} + C $$
\item$$\frac{21 z^{\frac{3}{4}}}{4} + \frac{z^{\frac{3}{2}}}{4} + \frac{7}{8 \sqrt[4]{z}} + C $$
\item$$- \frac{13}{18 \sqrt{y}} + C $$
\item$$- \frac{14}{3 z^{\frac{2}{3}}} + C $$
\item$$\frac{102 z^{\frac{8}{5}}}{25} + C $$
\item$$\frac{35 y^{\frac{7}{2}}}{8} + C $$
\item$$- \frac{15 z^{\frac{9}{4}}}{4} + C $$
\item$$- \frac{42 z^{\frac{7}{5}}}{5} - \frac{28 z^{\frac{4}{5}}}{5} + C $$
\item$$- \frac{7 z^{\frac{7}{2}}}{8} + \frac{25 z^{\frac{5}{2}}}{8} + C $$
        \end{enumerate}
        

        \section{Compute the integral}
        
        \begin{enumerate}
        \item$$\frac{1}{2} \log{\left (\tan^{2}{\left (\log{\left (z \right )} \right )} + 1 \right )} + C $$
\item$$- 8 z^{2} \sqrt{- 12 z^{2} - 11 z - 10} - \frac{22 z}{3} \sqrt{- 12 z^{2} - 11 z - 10} - \frac{20}{3} \sqrt{- 12 z^{2} - 11 z - 10} + C $$
\item$$- 7 \log^{2}{\left (z \right )} + C $$
\item$$\frac{19}{4} e^{4 y} - 2 e^{y} + C $$
\item$$\frac{1}{2} \log{\left (\tan^{2}{\left (\log{\left (y \right )} \right )} + 1 \right )} + C $$
\item$$\frac{390963 z^{8}}{2} - 905388 z^{7} + 2313288 z^{6} - 3787080 z^{5} + \frac{8771821 z^{4}}{2} - 3593194 z^{3} + 2083784 z^{2} - 774972 z + C $$
\item$$\frac{e^{2 y}}{2} + C $$
\item$$\frac{2 \left(e^{y}\right)^{\frac{3}{2}}}{3} + C $$
\item$$- \cos{\left (\sqrt{y} \right )} + C $$
\item$$\frac{20}{3} \sin^{3}{\left (z \right )} + C $$
        \end{enumerate}
        

    \end{document}
    